

Hint and Solution for Selected Exercises

D.N.Ghayatadak
Department of Mathematics
College of Engineering Pune-05
gdatta3.14@gmail.com
dng.maths@coep.ac.in

Acknowledgements: Thanks to all my colleagues of Mathematics Department of College of Engineering Pune-05. Specially Dr. C.M.Deshpande, Dr. P. M. Shinde, Mrs Ahilya Dhere, Dr. Megha Jain.

Conventions: In this course we take Laplace transform of function $f(t)$ which is defined for $t \geq 0$ as $\mathcal{L}\{f(t)\} = \int_0^\infty e^{-st} f(t) dt$ for those s for which the integral exists. Note that this Laplace transform is also known as unilateral Laplace transform or one-sided Laplace transform. So in this course we say Laplace transform of function $f(t)$ then it is understood that this unilateral Laplace transform of function $f(t)$ which is defined for $t \geq 0$. In the mathematics literature there is Bilateral Laplace transform (also known as two-sided Laplace transform) of function $g(t)$ which is defined for $t \in \mathbb{R}$ is defined as $\int_{-\infty}^\infty e^{-st} g(t) dt$. Also note that $\mathcal{L}^{-1}\{F(s)\} = f(t)$ means by default it is understood function $f(t)$ is defined for $t \geq 0$. For example $\mathcal{L}^{-1}\left\{\frac{s}{s^2+1}\right\} = \cos(t)$ (This means function $\cos(t)$ defined for $t \geq 0$)

Note: Capital letters in bracket is the choice for the correct answer.

$$1 \quad \mathcal{L}\{f(t)\} = \int_0^\infty e^{-st} f(t) dt \quad (B)$$

$$2 \quad \text{Observe that } \lim_{t \rightarrow \infty} e^{(t^2-kt)} \text{ is not finite} \quad (B)$$

$$3 \quad |\tan(t)| \rightarrow \infty \text{ as } t \rightarrow (2n+1)\pi/2 \text{ where } n \in \mathbb{N} \\ \text{Hence } \tan(t) \text{ is not of exponential order.} \quad (D)$$

$$4 \quad \text{We know that } \mathcal{L}(e^{at}) = \frac{1}{s-a} \text{ when } s > a \\ \text{Hence } \mathcal{L}(e^{-t}) = \frac{1}{s+1} \text{ for } s > -1 \quad (C)$$

$$5 \quad \mathcal{L}(e^{-2t}) = \frac{1}{s+2} \text{ for } s > -2 \quad (C)$$

$$6 \quad \mathcal{L}\{1 - e^{-2t}\} = \frac{1}{s} - \frac{1}{s+2} = \frac{2}{s(s+2)} \text{ for } s > 0, \\ \text{because } \mathcal{L}\{1\} = \frac{1}{s} \text{ for } s > 0 \text{ and } \mathcal{L}\{e^{-2t}\} = \frac{1}{s+2} \text{ for } s > -2 \text{ so we take maximum value of } s \\ \text{for which laplace transform exist.} \quad (A)$$

$$7 \quad \mathcal{L}\{\cos(\omega t)\} = \int_0^\infty e^{-st} \cos \omega t dt \\ \mathcal{L}\{\cos(\omega t)\} = \left[\frac{e^{-st}}{s^2 + \omega^2} (-s \cos \omega t + \omega \sin \omega t) \right]_0^\infty \\ \mathcal{L}\{\cos(\omega t)\} = \frac{s}{s^2 + \omega^2} \text{ for } s > 0 \quad (A)$$

$$8 \quad \text{We } \mathcal{L}\{\cosh(at)\} = \mathcal{L}\left\{\frac{e^{at} + e^{-at}}{2}\right\} \\ \mathcal{L}(\cosh(at)) = \frac{\mathcal{L}\{e^{at}\} + \mathcal{L}\{e^{-at}\}}{2} \\ \mathcal{L}\{\cosh(at)\} = \frac{1}{2} \left(\frac{1}{s-a} + \frac{1}{s+a} \right) s > a \text{ \& } s > -a \\ \mathcal{L}\{\cosh(at)\} = \frac{s}{s^2 - a^2} \text{ for } s > |a| \quad (A)$$

$$9 \quad \mathcal{L}\{2t+6\} = 2\mathcal{L}\{t\} + 6\mathcal{L}\{1\} = \frac{2}{s^2} + \frac{6}{s}; s > 0 \quad (C)$$

$$10 \quad \mathcal{L}\{t^2 + 2t + 1\} = \mathcal{L}\{t^2\} + 2\mathcal{L}\{t\} + \mathcal{L}\{1\} \\ \mathcal{L}\{t^2 + 2t + 1\} = \frac{2}{s^3} + \frac{2}{s^2} + \frac{1}{s} \text{ for } s > 0. \quad (D)$$

Having understood so far now we do not write the values of s for which Laplace transform exist.

$$11. \quad \mathcal{L}\{\sqrt{t}\} = \frac{\Gamma(\frac{1}{2} + 1)}{s^{3/2}} = \frac{\frac{1}{2}\Gamma(\frac{1}{2})}{s^{3/2}} = \frac{\sqrt{\pi}}{2s^{3/2}} \quad (C)$$

$$12. \quad \int_0^\infty \frac{e^{-st}}{\sqrt{t}} dt = \frac{1}{\sqrt{s}} \int_0^\infty e^{-u} u^{\frac{1}{2}-1} du \text{ (take } st = u) \\ \int_0^\infty \frac{e^{-st}}{\sqrt{t}} dt = \frac{\Gamma(1/2)}{\sqrt{s}} = \sqrt{\frac{\pi}{s}} \text{ for } s > 0$$

Alternative way to solve above integral is use $st = w^2$ substitution in above integral

$$\int_0^\infty \frac{e^{-st}}{\sqrt{t}} dt = \frac{2}{\sqrt{s}} \int_0^\infty e^{-w^2} dw = \sqrt{\frac{\pi}{s}} \quad (A)$$

$$13. \quad \mathcal{L}\left\{\frac{1}{\sqrt{\pi t}}\right\} = \frac{1}{\sqrt{\pi}} \mathcal{L}\left\{\frac{1}{\sqrt{t}}\right\} = \frac{1}{\sqrt{s}} \quad (B)$$

$$14 \quad \mathcal{L}\{6t^3 + 3\sin 4t\} = 6\mathcal{L}\{t^3\} + 3\mathcal{L}\{\sin 4t\} \\ \mathcal{L}\{6t^3 + 3\sin 4t\} = \frac{6 \cdot 3!}{s^4} + \frac{3 \cdot 4}{s^2 + 4^2} \\ \mathcal{L}\{6t^3 + 3\sin 4t\} = \frac{36}{s^4} + \frac{12}{s^2 + 4^2} \quad (A)$$

$$15 \quad \text{We know that } \sinh 5t = \frac{e^{5t} - e^{-5t}}{2} \\ 3e^{5t} \sinh 5t = \frac{3(e^{10t} - 1)}{2} = \frac{3e^{10t}}{2} - \frac{3}{2} \\ \mathcal{L}\{3e^{5t} \sinh 5t\} = \mathcal{L}\left\{\frac{3e^{10t}}{2}\right\} - \mathcal{L}\left\{\frac{3}{2}\right\} \\ \mathcal{L}\{3e^{5t} \sinh 5t\} = \frac{3}{2(s-10)} - \frac{3}{2s} = \frac{15}{s^2 - 10s} \quad (B)$$

$$16 \quad \mathcal{L}\{e^{-2t} \cos 4t\} = \frac{s+2}{(s+2)^2 + 16} \quad (D)$$

$$17 \quad \mathcal{L}\{e^{2t} \sin 5t\} = \frac{5}{(s-2)^2 + 5^2} = \frac{5}{s^2 - 4s + 29} \quad (A)$$

$$18 \quad \mathcal{L}\{te^t\} = -\frac{d}{ds} \left(\frac{1}{s-1} \right) = \frac{1}{(s-1)^2} \quad (B)$$

$$19 \quad \mathcal{L}\{t^n e^{-\alpha t}\} = \frac{n!}{(s+\alpha)^{n+1}} \quad (B)$$

$$20 \quad \text{Let } f(t) = 2 \cos 2t - \sin 2t, \quad \mathcal{L}\{f(t)\} = F(s). \\ \mathcal{L}\{e^{-t} f(t)\} = F(s+1) = \frac{2(s+1-1)}{(s+1)^2 + 4} \quad \text{So} \\ F(s) = \frac{2(s-1)}{s^2 + 4} \implies F(s-1) = \frac{2(s-2)}{(s-1)^2 + 4} \quad (A)$$

$$21 \quad \mathcal{L}\{t \cosh t\} = -\frac{d}{ds} \left(\frac{s}{s^2 - 1} \right) = \frac{s^2 + 1}{(s^2 - 1)^2} \quad (A)$$

$$22 \quad \text{Given that } \mathcal{L}\{f(t)\} = F(s) = \frac{1}{s^2 + s + 1} \\ \mathcal{L}\{tf(t)\} = -\frac{d}{ds} \left(\frac{1}{s^2 + s + 1} \right) = \frac{2s+1}{(s^2 + s + 1)^2} \\ \text{because } \mathcal{L}\{tf(t)\} = -F'(s) \quad (D)$$

$$23 \quad \mathcal{L} \left\{ \int_0^t f(\tau) d\tau \right\} = \frac{F(s)}{s} \quad (\text{Standard Theorem})(A)$$

$$24 \quad \text{Given } f(t) = \begin{cases} t & \text{if } 0 < t < 1 \\ 1 & \text{if } t > 1 \end{cases} \\ f(t) = t[u(t) - u(t-1)] + [u(t-1)] \\ f(t) = tu(t) - (t-1)u(t-1) \\ \mathcal{L}\{f(t)\} = \mathcal{L}\{tu(t) - (t-1)u(t-1)\} \\ \mathcal{L}\{f(t)\} = \mathcal{L}\{tu(t)\} - \mathcal{L}\{(t-1)u(t-1)\} \\ \mathcal{L}\{f(t)\} = \frac{e^{-0s}}{s^2} - \frac{e^{-s}}{s^2} = \frac{1 - e^{-s}}{s^2} \quad (B)$$

$$25 \quad \text{Take } g(x) = x \text{ So } g(x-3) = x-3 \text{ Using second shifting property } \mathcal{L}\{f(t-a)u(t-a)\} = e^{-st}F(s)$$

$$g(x-3)u(x-3) = \begin{cases} 0 & \text{for } x \leq 3 \\ x-3 & \text{for } x \geq 3 \end{cases}$$

$$\mathcal{L}\{g(x-3)u(x-3)\} = e^{-3s}\mathcal{L}\{x\} = e^{-3s}s^{-2} \quad (D)$$

$$26 \quad \mathcal{L}\{\sin kt\} = \frac{k}{s^2 + k^2} \neq \frac{s}{s^2 + k^2} \quad (C)$$

$$27 \quad \text{Unit-Step function defined as} \\ u(t-a) = \begin{cases} 0 & \text{if } t < a \\ 1 & \text{if } t > a \end{cases} \quad \text{where } a \geq 0 \\ \mathcal{L}\{u(t-a)\} = \int_0^\infty e^{-st}u(t-a)dt = \int_a^\infty e^{-st}dt \\ \mathcal{L}\{u(t-a)\} = \frac{e^{-as}}{s} \quad \text{for } s > 0 \quad (C)$$

$$28 \\ \mathcal{L}\{2[u(t) - u(t-1)]\} = 2\mathcal{L}\{u(t)\} - 2\mathcal{L}\{u(t-1)\} \\ \mathcal{L}\{2u(t) - 2u(t-1)\} = \frac{2e^{-0s}}{s} - \frac{2e^{-s}}{s} = \frac{2(1 - e^{-s})}{s} \\ \mathcal{L}\{2[u(t) - u(t-1)]\} = \frac{2(1 - e^{-s})}{s} \quad (C)$$

$$29 \quad \text{Given function can be written as combination of unit step function as } f(t) = u(t-3) - u(t-5).$$

$$\mathcal{L}\{f(t)\} = \mathcal{L}\{u(t-3)\} - \mathcal{L}\{u(t-5)\}$$

$$\mathcal{L}\{f(t)\} = \frac{e^{-3s}}{s} - \frac{e^{-5s}}{s} = \frac{e^{-3s} - e^{-5s}}{s}$$

$$\text{Alternative way is solve this question is use definition of Laplace transform } \mathcal{L}\{f(t)\} = \int_0^\infty e^{-st}f(t)dt = \int_3^5 e^{-st}dt = \frac{e^{-3s} - e^{-5s}}{s} \quad (A)$$

$$30 \quad \text{Let } f(t) = \begin{cases} 1 & \text{for } 0 \leq t \leq 1 \\ 0 & \text{otherwise} \end{cases} \text{ can be written as linear combination of unit step function as } f(t) = u(t) - u(t-1).$$

$$\mathcal{L}\{f(t)\} = \mathcal{L}\{u(t)\} - \mathcal{L}\{u(t-1)\}$$

$$\mathcal{L}\{f(t)\} = \frac{e^{-0s}}{s} - \frac{e^{-s}}{s}$$

$$\mathcal{L}\{f(t)\} = \frac{(1 - e^{-s})}{s} \quad \text{for } s > 0$$

$$\mathcal{L}\{f\} \cdot \mathcal{L}\{f\} = \frac{(1 - e^{-s})^2}{s^2} = \frac{1 - 2e^{-s} + e^{-2s}}{s^2}$$

$$\text{Convolution Theorem } \mathcal{L}\{f * f\} = \mathcal{L}\{f\} \cdot \mathcal{L}\{f\}$$

$$\mathcal{L}\{f * f\} = \frac{(1 - e^{-s})^2}{s^2} = \frac{1 - 2e^{-s} + e^{-2s}}{s^2}$$

$$f * f = \mathcal{L}^{-1} \left\{ \frac{1 - 2e^{-s} + e^{-2s}}{s^2} \right\}$$

$$f * f = \mathcal{L}^{-1} \left\{ \frac{1}{s^2} \right\} - 2\mathcal{L}^{-1} \left\{ \frac{e^{-s}}{s^2} \right\} + \mathcal{L}^{-1} \left\{ \frac{e^{-2s}}{s^2} \right\}$$

$$f * f = t - 2u(t-1)(t-1) + u(t-2)(t-2)$$

$$f * f = \begin{cases} t & 0 \leq t \leq 1 \\ t - 2(t-1) & 1 < t \leq 2 \\ t - 2(t-1) + (t-2) & 2 < t < \infty \end{cases}$$

$$f * f = \begin{cases} t & \text{for } 0 \leq t \leq 1 \\ 2 - t & \text{for } 1 < t \leq 2 \\ 0 & \text{for } 2 < t < \infty \end{cases}$$

$$x(t) = f * f \text{ hence } \mathcal{L}\{x(t)\} = \mathcal{L}\{f * f\} \quad (D)$$

$$31 \quad \mathcal{L}\{f(t)\} = \frac{1}{1 - e^{-sT}} \int_0^T e^{-st}f(t)dt$$

$$\mathcal{L}\{f(t)\} = \frac{1}{1 - e^{-s}} \left(\int_0^{1/2} e^{-st}f(t)dt + \int_{1/2}^1 e^{-st}f(t)dt \right)$$

$$\mathcal{L}\{f(t)\} = \frac{1}{1-e^{-s}} \left(\int_0^{1/2} e^{-st}(1)dt + \int_{1/2}^1 e^{-st}(0)dt \right)$$

$$\mathcal{L}\{f(t)\} = \frac{1}{1-e^{-s}} \left(\frac{e^{-st}}{-s} \right)_0^{1/2}$$

$$\mathcal{L}\{f(t)\} = \frac{1-e^{-s/2}}{s(1-e^{-s})}$$

$$\mathcal{L}\{f(t)\} = \frac{1-e^{-s/2}}{s(1-e^{s/2})(1+e^{-s/2})}$$

$$\mathcal{L}\{f(t)\} = \frac{1}{s(1+e^{-s/2})} \quad (B)$$

$$\begin{aligned} 32 \quad \mathcal{L}^{-1} \left\{ \frac{s+10}{(s+2)(s+20)} \right\} &= \mathcal{L}^{-1} \left\{ \frac{4/9}{s+2} + \frac{5/9}{s+20} \right\} \\ \mathcal{L}^{-1} \left\{ \frac{s+10}{(s+2)(s+20)} \right\} &= \frac{4}{9}e^{-2t} + \frac{5}{9}e^{-20t} \quad (C) \end{aligned}$$

$$\begin{aligned} 33 \quad \mathcal{L}^{-1} \left\{ \frac{s+1}{(s+4)(s-3)} \right\} &= \mathcal{L}^{-1} \left\{ \frac{3/7}{s+4} + \frac{4/7}{s-3} \right\} \\ \mathcal{L}^{-1} \left\{ \frac{s+1}{(s+4)(s-3)} \right\} &= \frac{3}{7}e^{-4t} + \frac{4}{7}e^{3t} \quad (B) \end{aligned}$$

$$34 \quad F(s) = \frac{1}{s^2(s+1)} = \frac{1}{s} \left[\frac{1}{s(s+1)} \right] = \frac{1}{s}G(s)$$

$$\text{where } G(s) = \frac{1}{s(s+1)} \quad \text{so } g(t) = 1 - e^{-t}$$

$$\text{Using } \mathcal{L} \left\{ \int_0^t g(t)dt \right\} = \frac{1}{s}G(s)$$

$$\mathcal{L}^{-1}\{F(s)\} = \mathcal{L}^{-1} \left\{ \frac{1}{s}G(s) \right\}$$

$$\mathcal{L}^{-1}\{F(s)\} = \int_0^t (1 - e^{-\tau})d\tau$$

$$\mathcal{L}^{-1}\{F(s)\} = -1 + t + e^{-t} \quad (A)$$

$$\begin{aligned} 35 \quad F(s) &= \frac{1}{s(s+1)} = \frac{s+1-s}{s(s+1)} = \frac{1}{s} - \frac{1}{(s+1)} \\ \mathcal{L}^{-1}\{F(s)\} &= \mathcal{L}^{-1} \left\{ \frac{1}{s} - \frac{1}{(s+1)} \right\} = 1 - e^{-t} \quad (C) \end{aligned}$$

$$\begin{aligned} 36 \quad \mathcal{L}^{-1} \left\{ \frac{s+3}{s^2+2s+1} \right\} &= \mathcal{L}^{-1} \left\{ \frac{s+1+2}{(s+1)^2} \right\} \\ \mathcal{L}^{-1} \left\{ \frac{s+3}{s^2+2s+1} \right\} &= \mathcal{L}^{-1} \left\{ \frac{1}{(s+1)} + \frac{2}{(s+1)^2} \right\} \\ \mathcal{L}^{-1} \left\{ \frac{s+3}{s^2+2s+1} \right\} &= e^{-t} + 2te^{-t} \quad (C) \end{aligned}$$

$$\begin{aligned} 37 \quad \frac{2s^2-4}{(s-3)(s^2-s-2)} &= \frac{A}{(s-3)} + \frac{B}{(s-2)} + \frac{C}{(s+1)} \\ 2s^2-4 &= A(s-2)(s+1) + B(s-3)(s+1) + C(s-3)(s-2) \\ \text{For } s=3, 2 \text{ and } -1 \text{ we get} \\ A &= \frac{7}{2}, B = \frac{-4}{3} \text{ and } C = \frac{-1}{6} \text{ respectively} \end{aligned}$$

$$\begin{aligned} \mathcal{L}^{-1}\{F(s)\} &= \frac{7}{2}\mathcal{L}^{-1} \left\{ \frac{1}{s-3} \right\} - \frac{4}{3}\mathcal{L}^{-1} \left\{ \frac{1}{s-2} \right\} - \\ \frac{1}{6}\mathcal{L}^{-1} \left\{ \frac{1}{s+1} \right\} &= \frac{7}{2}e^{3t} - \frac{4}{3}e^{2t} - \frac{1}{6}e^{-t} \quad (C) \end{aligned}$$

$$\begin{aligned} 38 \quad \mathcal{L}^{-1} \left\{ \frac{s+2}{(s+2)^2 + (10)^2} \right\} &= e^{-2t} \cos 10t = f(t) \\ \text{So } f(0) &= 1 \quad (C) \end{aligned}$$

$$\begin{aligned} 39 \quad F(s) &= \frac{2s+4-2}{s^2+4s+4+3} = \frac{2(s+2)-2}{(s+2)^2+3} \\ F(s) &= \frac{2(s+2)}{(s+2)^2+3} - \frac{2}{(s+2)^2+3} \\ \mathcal{L}^{-1}\{F(s)\} &= \mathcal{L}^{-1} \left\{ \frac{2(s+2)}{(s+2)^2+3} - \frac{2}{(s+2)^2+3} \right\} \\ f(t) &= 2e^{-2t} \left[\cos(\sqrt{3}t) - \frac{\sin(\sqrt{3}t)}{\sqrt{3}} \right] \\ f(0) &= 2 \quad \text{and} \quad \lim_{t \rightarrow \infty} f(t) = 0 \quad (B) \end{aligned}$$

$$\begin{aligned} 40 \quad F(s) &= \frac{1/2}{s} + \frac{1/2}{s+2} \\ \mathcal{L}^{-1}\{F(s)\} &= \mathcal{L}^{-1} \left\{ \frac{1/2}{s} + \frac{1/2}{s+2} \right\} \\ \mathcal{L}^{-1}\{F(s)\} &= \mathcal{L}^{-1} \left\{ \frac{1/2}{s} \right\} + \mathcal{L}^{-1} \left\{ \frac{1/2}{s+2} \right\} \\ f(t) &= \frac{1}{2}(1) + \frac{1}{2}e^{-2t} \quad \text{Alternative way is as follow} \\ \frac{s+1}{s(s+2)} &= \frac{1}{s(s+2)} + \frac{1}{s(s+2)} \\ \frac{s+1}{s+1} &= \frac{1}{(s+2)} + \frac{1}{s(s+2)} \\ \frac{s(s+2)}{s(s+2)} &= \frac{1}{(s+2)} + \frac{1}{2} \left(\frac{s+2-s}{s(s+2)} \right) \\ \frac{s+1}{s+1} &= \frac{1}{(s+2)} + \frac{1}{2s} \\ \frac{s(s+2)}{s(s+2)} &= \frac{1}{2(s+2)} + \frac{1}{2s} \\ \mathcal{L}^{-1} \left\{ \frac{s+1}{s(s+2)} \right\} &= \frac{1+e^{-2t}}{2} \\ f(0) &= 1 \quad \text{and} \quad \lim_{t \rightarrow \infty} f(t) = 1/2 \quad (B) \end{aligned}$$

$$41 \quad \text{Given } y'' + y = 6 \cos(2x); \quad y(0) = 3, \quad y'(0) = 1$$

$$\mathcal{L}\{y'' + y\} = \mathcal{L}\{6 \cos(2x)\}$$

$$\mathcal{L}\{y''\} + \mathcal{L}\{y\} = 6\mathcal{L}\{\cos(2x)\}$$

$$s^2\mathcal{L}\{y\} - sy(0) - y'(0) + \mathcal{L}\{y\} = \frac{6s}{s^2+4}$$

$$(s^2+1)\mathcal{L}\{y\} - 3s - 1 = \frac{6s}{s^2+4}$$

$$(s^2+1)\mathcal{L}\{y\} = \frac{6s}{s^2+4} + (3s+1)$$

$$\mathcal{L}\{y\} = \frac{6s}{(s^2+4)(s^2+1)} + \frac{(3s+1)}{(s^2+1)}$$

$$Y(s) = \frac{6s + (3s+1)(s^2+4)}{(s^2+4)(s^2+1)}$$

$$Y(1) = \frac{13}{5} \quad (B)$$

42 Given $u'' + 2u' + u = 1$; $u(0) = 0$, $u'(0) = 5$.

$$\mathcal{L}\{u'' + 2u' + u\} = \mathcal{L}\{1\}$$

$$\mathcal{L}\{u''\} + \mathcal{L}\{u'\} + \mathcal{L}\{u\} = \mathcal{L}\{1\}$$

$$(s^2 + 2s + 1)\mathcal{L}\{u\} - su(0) - u'(0) - 2u(0) = \frac{1}{s}$$

$$(s^2 + 2s + 1)\mathcal{L}\{u\} = \frac{1}{s} + 5$$

$$U(s) = \frac{1 + 5s}{s(s^2 + 2s + 1)} \quad (B)$$

43 $y'' + 5y' + 6y = u(t) - u(t - 2)$

Taking Laplace Transform on both side

$$\mathcal{L}\{y'' + 5y' + 6y\} = \mathcal{L}\{u(t) - u(t - 2)\}$$

$$s^2\mathcal{L}\{y(t)\} + 5s\mathcal{L}\{y(t)\} + 6\mathcal{L}\{y(t)\} = \frac{e^{-0s}}{s} - \frac{e^{-2s}}{s}$$

$$(s^2 + 5s + 6)Y(s) = \frac{1 - e^{-2s}}{s}$$

$$Y(s) = \frac{1 - e^{-2s}}{s(s^2 + 5s + 6)} \quad (B)$$

44 We can rewrite $f(x)$ as $f(x) = 2[u(x) - u(x - 1)]$

So $y' + y = 2u(x) - 2u(x - 1)$; $y(0) = 0$.

Take Laplace Transform on both side

$$\mathcal{L}\{y' + y\} = \mathcal{L}\{2u(x) - 2u(x - 1)\}$$

$$\mathcal{L}\{y'\} + \mathcal{L}\{y\} = 2\mathcal{L}\{u(x)\} - 2\mathcal{L}\{u(x - 1)\}$$

$$s\mathcal{L}\{y\} - y(0) + \mathcal{L}\{y\} = \frac{2e^{-0s}}{s} - \frac{2e^{-s}}{s}$$

$$(s + 1)Y(s) = \frac{2(1 - e^{-s})}{s}$$

$$Y(s) = \frac{2(1 - e^{-s})}{s(s + 1)}$$

$$Y(s) = 2\left(\frac{1}{s} - \frac{1}{s + 1}\right) - 2e^{-s}\left(\frac{1}{s} - \frac{1}{s + 1}\right)$$

Now take Inverse Laplace Transform on both side,

$$y(x) = \mathcal{L}^{-1}\left\{\frac{2}{s} - \frac{2}{s + 1} - \frac{2e^{-s}}{s} + \frac{2e^{-s}}{s + 1}\right\}$$

$$y(x) = 2 - 2e^{-x} - 2u(x - 1)(1) + 2u(x - 1)e^{-(x-1)}$$

$$y(x) = \begin{cases} 2 - 2e^{-x} & \text{for } 0 \leq x \leq 1 \\ 2 - 2e^{-x} - 2 + 2e^{-(x-1)} & \text{for } x \geq 1 \end{cases}$$

$$y(x) = \begin{cases} 2(1 - e^{-x}) & \text{for } 0 \leq x < 1 \\ (2e - 2)e^{-x} & \text{for } x \geq 1 \end{cases} \quad (A)$$

45 Given $y'' + 2y' + 5y = 3e^{-t} \sin t$; $y(0) = 0$, $y'(0) = 3$

$$\mathcal{L}\{y'' + 2y' + 5y\} = \mathcal{L}\{3e^{-t} \sin t\}$$

$$\mathcal{L}\{y''\} + 2\mathcal{L}\{y'\} + 5\mathcal{L}\{y\} = \mathcal{L}\{3e^{-t} \sin t\}$$

$$(s^2 + 2s + 5)\mathcal{L}\{y\} - 3 = \frac{3}{(s + 1)^2 + 1}$$

$$Y(s) = \frac{3[(s + 1)^2 + 1] + 3}{[(s + 1)^2 + 1][(s + 1)^2 + 2^2]}$$

$$Y(s) = \frac{3}{[(s + 1)^2 + 2^2]} + \frac{3}{[(s + 1)^2 + 2^2][(s + 1)^2 + 2^2]}$$

$$Y(s) = \frac{3}{[(s + 1)^2 + 2^2]} + \frac{[s^2 + 2s + 5] - [s^2 + 2s + 2]}{[(s + 1)^2 + 1][(s + 1)^2 + 2^2]}$$

$$Y(s) = \frac{2}{[(s + 1)^2 + 2^2]} + \frac{1}{[(s + 1)^2 + 1^2]}$$

$$y(t) = e^{-t}(\sin(2t) + \sin(t)) \quad (B)$$

46 Note that $\sin(t - 2\pi) = \sin(t)$

$$\mathcal{L}\{y'' + y\} = \mathcal{L}\{\sin(t)u(t - 2\pi)\}$$

$$\mathcal{L}\{y'' + y\} = \mathcal{L}\{\sin(t - 2\pi)u(t - 2\pi)\}$$

$$(s^2 + 1)\mathcal{L}\{y\} - s - 1 = \frac{e^{-2\pi s}}{s^2 + 1}$$

$$\mathcal{L}\{y\} = \frac{e^{-2\pi s}}{(s^2 + 1)^2} + \frac{s + 1}{s^2 + 1} \quad (?)$$

48 $\mathcal{L}\{y'(t) + 5y(t)\} = \mathcal{L}\{u(t)\}$

$$s\mathcal{L}\{y(t)\} - y(0) + 5\mathcal{L}\{y(t)\} = \frac{1}{s}$$

$$(s + 5)Y(s) = \frac{s + 1}{s}$$

$$Y(s) = \frac{s + 1}{s(s + 5)} = \frac{1/5}{s} + \frac{4/5}{s + 5} = \frac{0 \cdot 2}{s} + \frac{0 \cdot 8}{s + 5}$$

$$y(t) = \mathcal{L}^{-1}\left\{\frac{0 \cdot 2}{s} + \frac{0 \cdot 8}{s + 5}\right\} = 0.2 + 0.8e^{-5t} \quad (A)$$

49

$$\mathcal{L}\left\{\frac{dy}{dt} + y(t)\right\} = \mathcal{L}\{\delta(t)\}$$

$$\mathcal{L}\left\{\frac{dy}{dt}\right\} + \mathcal{L}\{y(t)\} = \mathcal{L}\{\delta(t)\}$$

$$s\mathcal{L}\{y\} - y(0) + \mathcal{L}\{y\} = 1$$

$$(s + 1)Y(s) = 1$$

$$Y(s) = \frac{1}{s + 1}$$

$$\mathcal{L}^{-1}\{Y(s)\} = \mathcal{L}^{-1}\left\{\frac{1}{s + 1}\right\}$$

$$y(t) = e^{-t} \quad \text{for } t \geq 0$$

$$y(t) = e^{-t}u(t) \quad (D)$$

52 Given system of differential eq. can be written as

$$\begin{array}{l|l} x' = -x, & y' = -2y \text{ with } x(0) = 1, y(0) = -1 \\ x' = -x; & x(0) = 1 \end{array} \quad \begin{array}{l} y' = -2y; y(0) = -1 \end{array}$$

$$\mathcal{L}\{x'\} = \mathcal{L}\{-x\}$$

$$\mathcal{L}\{y'\} = \mathcal{L}\{-2y\}$$

$$(s + 1)X(s) = x(0)$$

$$(s + 2)Y(s) = y(0)$$

$$X(s) = \frac{1}{s + 1}$$

$$Y(s) = \frac{-1}{s + 2}$$

$$x(t) = \mathcal{L}^{-1}\left\{\frac{1}{s + 1}\right\}$$

$$y(t) = \mathcal{L}^{-1}\left\{\frac{-1}{s + 2}\right\}$$

$$x(t) = e^{-t} \quad \left| \quad y(t) = -e^{-2t} \quad (C) \right.$$

53 Given equation $y(x) = x^3 + \sin t * y(t)$

$$\begin{aligned}
 \mathcal{L}\{y(x)\} &= \mathcal{L}\{x^3\} + \mathcal{L}\{\sin t * y(t)\} \\
 Y(s) &= \frac{3!}{s^4} + \mathcal{L}\{\sin t\} \cdot \mathcal{L}\{y(t)\} \\
 Y(s) &= \frac{6}{s^4} + \frac{Y(s)}{s^2 + 1} \\
 \left(1 - \frac{1}{s^2 + 1}\right) Y(s) &= \frac{6}{s^4} \\
 \left(\frac{s^2}{s^2 + 1}\right) Y(s) &= \frac{6}{s^4} \\
 Y(s) &= \frac{6}{s^4} \frac{s^2 + 1}{s^2} \\
 Y(s) &= 6 \left(\frac{1}{s^4} + \frac{1}{s^6} \right) \\
 y(t) &= \mathcal{L}^{-1} \left\{ 6 \left(\frac{1}{s^4} + \frac{1}{s^6} \right) \right\} \\
 y(t) &= 6 \mathcal{L}^{-1} \left\{ \frac{1}{s^4} \right\} + 6 \mathcal{L}^{-1} \left\{ \frac{1}{s^6} \right\} \\
 y(t) &= 6 \left(\frac{t^3}{3!} + \frac{t^5}{5!} \right) = t^3 + \frac{t^5}{20} \\
 y(1) &= 1 + \frac{1}{20} = \frac{21}{20} \quad (D)
 \end{aligned}$$

54 Given equation $\varphi(x) = x + \varphi(x) * \sin(x)$

$$\begin{aligned}
 \mathcal{L}\{\varphi(x)\} &= \mathcal{L}(x) + \mathcal{L}\{\varphi(x) * \sin(x)\} \\
 \mathcal{L}\{\varphi(x)\} &= \mathcal{L}(x) + \mathcal{L}\{\varphi(x)\} \cdot \mathcal{L}\{\sin(x)\} \\
 \mathcal{L}\{\varphi(x)\} &= \frac{1}{s^2} + \frac{1}{s^2 + 1} \mathcal{L}\{\varphi(x)\} \\
 \mathcal{L}\{\varphi(x)\} \left(1 - \frac{1}{s^2 + 1}\right) &= \frac{1}{s^2} \\
 \mathcal{L}\{\varphi(x)\} &= \frac{s^2 + 1}{s^4} \\
 \varphi(x) &= \mathcal{L}^{-1} \left\{ \frac{1}{s^2} \right\} + \mathcal{L}^{-1} \left\{ \frac{1}{s^4} \right\} \\
 \varphi(x) &= x + \frac{x^3}{3!} \quad (C)
 \end{aligned}$$

$$\begin{aligned}
 55 \quad f * g &= \int_0^t f(\tau) g(t - \tau) d\tau \\
 f(t) &= e^{-t} \text{ and } g(t) = e^{-2t} \text{ for } t > 0 \\
 f * g &= \int_0^t e^{-\tau} e^{-2(t-\tau)} d\tau \\
 f * g &= e^{-2t} \int_0^t e^{\tau} d\tau = e^{-t} - e^{-2t}
 \end{aligned}$$

Alternative way to solve this problem is use

convolution theorem

$$\begin{aligned}
 \mathcal{L}\{e^{-t} * e^{-2t}\} &= \mathcal{L}\{e^{-t}\} \mathcal{L}\{e^{-2t}\} \\
 \mathcal{L}\{e^{-t} * e^{-2t}\} &= \frac{1}{(s+1)(s+2)} \\
 e^{-t} * e^{-2t} &= \mathcal{L}^{-1} \left\{ \frac{1}{(s+1)(s+2)} \right\} \\
 e^{-t} * e^{-2t} &= \mathcal{L}^{-1} \left\{ \frac{(s+2) - (s+1)}{(s+1)(s+2)} \right\} \\
 e^{-t} * e^{-2t} &= \mathcal{L}^{-1} \left\{ \frac{1}{s+1} \right\} - \mathcal{L}^{-1} \left\{ \frac{1}{s+2} \right\} \\
 e^{-t} * e^{-2t} &= e^{-t} - e^{-2t} \quad (A)
 \end{aligned}$$

58

$$\begin{aligned}
 \mathcal{L}\{e^{-t^2}\} &= \int_0^\infty e^{-t^2} e^{-st} dt = \int_0^\infty e^{-(t^2+st)} dt \\
 \mathcal{L}\{e^{-t^2}\} &= \int_0^\infty e^{-(t^2+st+\frac{s^2}{4}-\frac{s^2}{4})} dt \\
 \mathcal{L}\{e^{-t^2}\} &= \int_0^\infty e^{(-t+\frac{s}{2})^2} e^{\frac{s^2}{4}} dt = e^{\frac{s^2}{4}} \int_0^\infty e^{-(t+\frac{s}{4})^2} dt
 \end{aligned}$$

Take $t + \frac{s}{2} = u$ so $dt = du$

$$\begin{aligned}
 \mathcal{L}\{e^{-t^2}\} &= e^{\frac{s^2}{4}} \int_{s/2}^\infty e^{-u^2} du \\
 \mathcal{L}\{e^{-t^2}\} &= e^{\frac{s^2}{4}} \left[\int_0^{s/2} e^{-u^2} du + \int_{s/2}^\infty e^{-u^2} du - \int_0^{s/2} e^{-u^2} du \right] \\
 \mathcal{L}\{e^{-t^2}\} &= e^{\frac{s^2}{4}} \left[\int_0^\infty e^{-u^2} du - \int_0^{s/2} e^{-u^2} du \right]
 \end{aligned}$$

Recall: The Error function $\text{erf}(x)$ is defined

by $\text{erf}(x) = \frac{2}{\sqrt{\pi}} \int_0^x e^{-t^2} dt$. The complementary error function defined as $1 - \text{erfc}(x) = \frac{2}{\sqrt{\pi}} \int_x^\infty e^{-t^2} dt$ Note that $\text{erf}(x) + \text{erfc}(x) = 1$.

since $\int_{-\infty}^\infty e^{-x^2} dx = \sqrt{\pi}$

$$\begin{aligned}
 \mathcal{L}\{e^{-t^2}\} &= e^{\frac{s^2}{4}} \left[\frac{\sqrt{\pi}}{2} - \frac{\sqrt{\pi}}{2} \text{erf}\left(\frac{s}{2}\right) \right] \\
 \mathcal{L}\{e^{-t^2}\} &= e^{\frac{s^2}{4}} \frac{\sqrt{\pi}}{2} \left[1 - \text{erf}\left(\frac{s}{2}\right) \right] = \frac{\sqrt{\pi}}{2} e^{\frac{s^2}{4}} \text{erfc}\left(\frac{s}{2}\right)
 \end{aligned}$$

65 Please refer solution of question no: 30

If you found any mistake(s) please report me at dng.maths@coep.ac.in ■